SepLib/HImpl.lean
@@ -1,0 +1,94 @@
+import SepLib.HProp
+
+namespace HProp
+
+def entails (P Q : HProp) : Prop :=
+  ∀ (h : Heap), P h → Q h
+
+infix:50 " ⊢ " => entails
+
+@[refl]
+theorem entails_refl (P : HProp) :
+    P ⊢ P := by
+  intro h hP
+  assumption
+
+instance : IsRefl HProp entails := ⟨entails_refl⟩
+
+theorem entails_trans (P Q R : HProp) :
+    P ⊢ Q →
+    Q ⊢ R →
+    P ⊢ R := by
+  intros hPQ hQR h hP
+  apply hQR
+  apply hPQ
+  assumption
+
+instance : IsTrans HProp entails := ⟨entails_trans⟩
+
+theorem entails_antisymm (P Q : HProp) :
+    P ⊢ Q →
+    Q ⊢ P →
+    P = Q := by
+  intro hPQ hQP
+  ext
+  constructor <;> intro
+  · apply hPQ
+    assumption
+  · apply hQP
+    assumption
+
+instance : IsAntisymm HProp entails := ⟨entails_antisymm⟩
+
+theorem entails_frame_left {P Q : HProp} (R : HProp) :
+    P ⊢ Q →
+    (R ∗* P) ⊢ (R ∗* Q) := by
+  rintro hPQ h ⟨h1, h2, rfl, d, hR, hP⟩
+  star_exists h1, h2
+
+theorem entails_frame_right {P Q : HProp} (R : HProp) :
+    P ⊢ Q →
+    (P ∗* R) ⊢ (Q ∗* R) := by
+  intro
+  conv => args; all_goals rw [star_comm]
+  apply entails_frame_left
+  assumption
+
+theorem entails_star_pure_right {P : Prop} {H1 H2 : HProp} :
+    P → (H1 ⊢ H2) →
+    H1 ⊢ (H2 ∗* ⟦ P ⟧) := by
+  intro hP hentails h hH
+  star_exists h, ∅
+  exists hP
+
+theorem entails_star_pure_left {P : Prop} {H1 H2 : HProp} :
+    (P → H1 ⊢ H2) →
+    (⟦ P ⟧ ∗* H1) ⊢ H2 := by
+  rintro hentails h ⟨h1, h2, rfl, d, ⟨hP, rfl⟩, hH⟩
+  rw [Heap.empty_union]
+  apply hentails hP
+  assumption
+
+theorem entilas_exists_right {α : Sort*} {x : α} {J : α → HProp} {H : HProp} :
+    (H ⊢ J x) →
+    H ⊢ (∃ x, J x) := by
+  intro hentails h hH
+  exists x
+  simp
+  apply hentails
+  assumption
+
+theorem entails_exists_left {α : Sort*} {J : α → HProp} {H : HProp} :
+    (∀ x, J x ⊢ H) →
+    (∃ x, J x) ⊢ H := by
+  intro hentails h ⟨x, hJ⟩
+  apply hentails x
+  assumption
+
+theorem star_points_to_same_loc {l : Loc} {v1 v2 : Val} :
+    (l ↦ v1 ∗* l ↦ v2) ⊢ ⟦ False ⟧ := by
+  rintro h ⟨h1, h2, rfl, d, rfl, rfl⟩
+  have := Heap.disjoint_singleton.mp d
+  contradiction
+
+end HProp
